"Fix" prepare_procedures_entrypoints_after_linking
Following the sane pattern of the memory separation lemma, correct the
definitions required for the result on entrypoints, and move the last
Machine outtake from Composition to its proper location. As expected,
the proofs end up being extremely similar.

Intermediate/Machine.v
@@ -774,11 +774,106 @@ Proof.
     + simpl. rewrite Hmainp Hmainc. reflexivity. (* Easy case. *)
 Admitted. (* Grade 2. A few easy admits and "the issue". *)
 
+(*
 Definition prepare_procedures_entrypoints (p: program) (mem: Memory.t) : EntryPoint.t :=
   let '(_, _, entrypoints) := prepare_procedures p mem in
   entrypoints.
+*)
 
-(* Lemma placeholder: prepare_procedures_entrypoints_after_linking *)
+Definition prepare_procedures_entrypoints (p: program) : EntryPoint.t :=
+  let '(_, _, entrypoints) := prepare_procedures_initial_memory p in
+  entrypoints.
+
+(* RB: TODO: Observe this is the exact same proof as the _memory_ analog! *)
+Theorem prepare_procedures_entrypoints_after_linking:
+  forall p c,
+    well_formed_program p ->
+    well_formed_program c ->
+    linkable (prog_interface p) (prog_interface c) ->
+    linkable_mains p c ->
+    prepare_procedures_entrypoints (program_link p c) =
+    unionm (prepare_procedures_entrypoints p)
+           (prepare_procedures_entrypoints c).
+Proof.
+  intros p c Hwfp Hwfc Hlinkable Hmains.
+  unfold prepare_procedures_entrypoints,
+         prepare_procedures_initial_memory, prepare_procedures_initial_memory_aux.
+  (* Peel off the top-level maps. *)
+  rewrite <- mapm_unionm.
+  apply mapm_eq.
+  apply eq_fmap. intros Cid.
+  (* Case analysis on component provenance after some common preprocessing. *)
+  destruct (Cid \in domm (prog_interface p)) eqn:Hp;
+    destruct (Cid \in domm (prog_interface c)) eqn:Hc.
+  - admit. (* Contra. *)
+  - rewrite unionmE.
+    rewrite !mkfmapfE.
+    rewrite Hp Hc.
+    assert (Hpc : Cid \in domm (prog_interface (program_link p c)))
+      by (by apply in_domm_program_link).
+    rewrite Hpc.
+    assert ((elementsm (odflt emptym ((prog_procedures (program_link p c)) Cid))) =
+            (elementsm (odflt emptym ((prog_procedures p) Cid))))
+      as Helts by admit.
+    rewrite Helts.
+    assert (ComponentMemory.prealloc (odflt emptym ((prog_buffers (program_link p c)) Cid)) =
+            ComponentMemory.prealloc (odflt emptym ((prog_buffers p) Cid)))
+      as Hprealloc by admit.
+    rewrite Hprealloc.
+    simpl.
+    unfold reserve_component_blocks.
+    rewrite unionmE.
+    assert (exists x, (prog_interface p) Cid = Some x)
+      as [Cid_int Hp'] by (by apply /dommP).
+    rewrite Hp'.
+    simpl.
+    destruct (prog_main p) as [mainp |] eqn:Hmainp;
+      destruct (prog_main c) as [mainc |] eqn:Hmainc.
+    + easy. (* Contra. *)
+    + reflexivity.
+    + destruct Cid as [| n].
+      * (* It does not make sense that Component.main is in p,
+           but main is defined in c. *)
+        admit.
+      * reflexivity.
+    + reflexivity. (* Easy case. *)
+  - (* RB: TODO: Refactor symmetric case to last one. *)
+    rewrite unionmE.
+    rewrite !mkfmapfE.
+    rewrite Hp Hc.
+    assert (Hpc : Cid \in domm (prog_interface (program_link p c)))
+      by admit.
+    rewrite Hpc.
+    assert ((elementsm (odflt emptym ((prog_procedures (program_link p c)) Cid))) =
+            (elementsm (odflt emptym ((prog_procedures c) Cid))))
+      as Helts by admit.
+    rewrite Helts.
+    assert (ComponentMemory.prealloc (odflt emptym ((prog_buffers (program_link p c)) Cid)) =
+            ComponentMemory.prealloc (odflt emptym ((prog_buffers c) Cid)))
+      as Hprealloc by admit.
+    rewrite Hprealloc.
+    simpl.
+    unfold reserve_component_blocks.
+    rewrite unionmE.
+    assert ((prog_interface p) Cid = None)
+      as Hp' by (by apply /dommPn; rewrite Hp).
+    rewrite Hp'.
+    assert (exists x, (prog_interface c) Cid = Some x)
+      as [Cid_int Hc'] by (by apply /dommP).
+    rewrite Hc'.
+    destruct (prog_main p) as [mainp |] eqn:Hmainp;
+      destruct (prog_main c) as [mainc |] eqn:Hmainc.
+    + (* Contra. *)
+      unfold linkable_mains in Hmains.
+      rewrite Hmainp Hmainc in Hmains.
+      discriminate.
+    + simpl. rewrite Hmainp Hmainc.
+      destruct Cid as [| n].
+      * (* Should-be contra. *) admit.
+      * reflexivity.
+    + simpl. rewrite Hmainp Hmainc. reflexivity.
+    + simpl. rewrite Hmainp Hmainc. reflexivity. (* Easy case. *)
+Admitted. (* Grade 2. A few easy admits and "the issue". *)
 
 Lemma interface_preserves_closedness_r :
   forall p1 p2 p2',
